Wrote more theorems that related the fast version of the trellis calculating functions to the slow version. Modified the fast version of the function which calculates errors in the trellis so that it has a sensible definition when we are leading to the zeroth time-step. Wrote helper theorem saying that all transitions calculated when calculating the transitions leading to a particular state are contained in the set of all valid transitions.

convolutional_codesScript.sml
@@ -1108,6 +1108,20 @@ Definition transition_inverse_def:
   FILTER (λorgn. (m.transition_fn orgn).destination = dest) (all_transitions m)
 End
 
+Theorem transition_inverse_mem_all_transitions_set[simp]:
+  ∀m s r.
+  MEM r (transition_inverse m s) ⇒
+  r ∈ all_transitions_set m
+Proof
+  rpt strip_tac
+  >> gvs[transition_inverse_def]
+  >> gvs[MEM_FILTER]
+  >> gvs[all_transitions_set_def]
+  >> gvs[all_transitions_def]
+  >> gvs[all_transitions_helper_def]
+  >> gvs[MEM_GENLIST]
+QED
+
 Theorem transition_inverse_mem[simp]:
   ∀m s r.
   MEM r (transition_inverse m s) ⇒
@@ -1365,7 +1379,7 @@ End
 (* Invalid at time-step 0 because there is no previous row in this case.      *)
 (* -------------------------------------------------------------------------- *)
 Definition get_num_errors_calculate_no_prev_data_def:
-  get_num_errors_calculate_no_prev_data m bs 0 r = ARB ∧
+  get_num_errors_calculate_no_prev_data m bs 0 r = (if (vd_step_tran m r = 0) then N0 else INFINITY) ∧
   get_num_errors_calculate_no_prev_data m bs (SUC t) r = get_num_errors_calculate m bs (SUC t) (viterbi_trellis_row m bs t) r
 End
 
@@ -1700,11 +1714,43 @@ Theorem get_num_errors_calculate_slow_get_num_errors_calculate:
        r.origin < m.num_states ⇒
        get_num_errors_calculate_slow m bs (SUC t) r = get_num_errors_calculate m bs (SUC t) (viterbi_trellis_row m bs t) r
 Proof
+  gvs[get_num_errors_calculate_slow_get_num_errors_calculate_no_prev_data, get_num_errors_calculate_no_prev_data_def]
+QED
+
+
+Theorem get_better_origin_slow_get_better_origin:
+  ∀m bs t r1 r2.
+  wfmachine m ∧
+  r1.origin < m.num_states ∧
+  r2.origin < m.num_states ⇒
+  get_better_origin_slow m bs (SUC t) r1 r2 = get_better_origin m bs (SUC t) (viterbi_trellis_row m bs t) r1 r2
+Proof
+  rpt strip_tac
+  >> gvs[get_better_origin_slow_def, get_better_origin_def]
+  >> gvs[get_num_errors_calculate_slow_get_num_errors_calculate]
 QED
 
 Theorem best_origin_slow_best_origin:
-  best_origin_slow m bs t s = best_origin m bs t previous_row s  
+  ∀m bs t s.
+  wfmachine m ∧
+  s < m.num_states ⇒
+  best_origin_slow m bs (SUC t) s = best_origin m bs (SUC t) (viterbi_trellis_row m bs t) s  
 Proof
+  rpt strip_tac
+  >> gvs[best_origin_slow_def, best_origin_def]
+  >> irule FOLDR_DOMAIN
+  >> MEM_DONOTEXPAND_TAC
+  >> qexists ‘all_transitions_set m’
+  >> gvs[]
+  >> rpt strip_tac
+  >- (DEP_PURE_ONCE_REWRITE_TAC[get_better_origin_slow_get_better_origin]
+      >> gvs[all_transitions_set_def]
+     )
+  >- (gvs[get_better_origin_slow_def]
+      >> qmatch_goalsub_abbrev_tac ‘if b then _ else _’
+      >> Cases_on ‘b’ >> gvs[])
+  >> MEM_DOEXPAND_TAC
+  >> gvs[]
 QED         
 
 Theorem viterbi_trellis_node_slow_viterbi_trellis_node_no_prev_data:
@@ -3341,7 +3387,6 @@ Proof
   rpt strip_tac
   >> 
 QED*)
-
 
 Theorem code_to_path_helper_length:
   ∀m bs s.
